\documentclass{unswmaths}

\usepackage{unswshortcuts}

\begin{document}

\subject{Measure Theory}
\author{Edward McDonald}
\title{Present for Stuart}
\studentno{3375335}


\setlength\parindent{0pt}


\newcommand{\Bor}{\mathcal{B}}
\newcommand{\sdiff}{\bigtriangleup}
\newcommand{\Expect}{{\rm I\kern-.3em E}}
\newcommand{\Prob}{{\rm I\kern-.3em P}}
\newcommand{\Log}{\operatorname{Log}}


\unswtitle{}




\begin{lemma}
\label{stuart}
    Suppose that $q_n \rightarrow \lambda \in \Cplx$ is a sequence of complex
    numbers. Then
    \begin{equation*}
        \lim_{n\rightarrow\infty} \left(1+\frac{q_n}{n}\right)^n = e^{\lambda}
    \end{equation*} 
\end{lemma}
\begin{proof}
    Fix $n$ large enough such that $|q_n|/n < 1/2$.
    
    Since $q_n$ is a convergent sequence, it is bounded. Let $M$
    be large enough such that $|q_n| < M$ for all $n$.
    
    Re-write $\left(1+\frac{q_n}{n}\right)^n$ as $\exp(n\Log(1+\frac{q_n}{n}))$.
    
    The branch of the logarithm taken here is complex differentiable
    in the set $\Cplx\setminus(-\infty,0]$. Since $|q_n|/n < 1$, the above is valid.
    
    So it is sufficient to show that,
    \begin{equation*}
        \lim_{n\rightarrow\infty} n\Log\left(1+\frac{q_n}{n}\right) = \lambda
    \end{equation*}
    
    The $z\mapsto \Log(1+z)$ function is complex differentiable in the unit disc,
    and has a power series representation 
    \begin{equation*}
        \Log(1+z) = \sum_{k=1}^\infty (-1)^{k-1}\frac{z^k}{k}
    \end{equation*}
    which converges uniformly on compact subsets of the open unit disc $\{z\in \Cplx\;:\;|z| < 1\}$.
    
    Now, since $|q_n|/n < 1$, we have
    \begin{equation*}
        n\Log(1+\frac{q_n}{n}) = q_n+\sum_{k=2}^\infty (-1)^{k-1}\frac{q_n^k}{kn^{k-1}}
    \end{equation*}
    
    Now we consider the tail of the left hand side, let
    \begin{equation*}
        L_n := \sum_{k=2}^\infty (-1)^{k-1} \frac{q_n^k}{kn^{k-1}}
    \end{equation*}
    
    By the triangle inequality,
    \begin{equation*}
        |L_n| \leq \sum_{k=2}^\infty \frac{M^k}{kn^{k-1}}
    \end{equation*}
    Thus,
    \begin{align*}
        |L_n| &\leq M\sum_{k=1}^\infty \left(\frac{M}{n}\right)^k\\
        &= M\frac{M/n}{(1-M/n)}
    \end{align*}
    Hence, $L_n\rightarrow 0$ as $n\rightarrow\infty$.
    Thus, the limit
    \begin{equation*}
        \lim_{n\rightarrow\infty} n\Log(1+\frac{q_n}{n})
    \end{equation*}
    exists, and equals $\lim_{n\rightarrow\infty}q_n = \lambda$.
    
    Hence, the limit
    \begin{equation*}
        \lim_{n\rightarrow\infty}\left(1+\frac{q_n}{n}\right)^n
    \end{equation*}
    exists, and equals $e^\lambda$.
\end{proof}

Now we let $\{p_n\}_{n=1}^\infty$ be a monotone decreasing sequence, such
that $np_n \rightarrow \lambda$. We let $\mu_n = \mathrm{Bin}(n,p_n)$.
\begin{theorem}
    There is weak convergence, $\mu_n\rightarrow\nu$.
\end{theorem}
\begin{proof}
    By L\'evy's continuity theorem, it is sufficient to show pointwise convergence
    of characteristic functions, $\hat{\mu}_n(u)\rightarrow \hat{\nu}(u)$
    for all $u$. That is, we must show
    \begin{equation*}
        \lim_{n\rightarrow\infty} (1-p_n+p_ne^{iu})^n = \exp(\lambda(e^{iu}-1)).
    \end{equation*}    
    
    Rewrite $\hat{\mu}_n(u)$ as
    \begin{equation*}
        \left(1+\frac{np_n(e^{iu}-1)}{n}\right)^n
    \end{equation*}
    Now by lemma \ref{stuart}, we see
    \begin{equation*}
        \lim_{n\rightarrow\infty} \hat{\mu}_n(u) = \exp(\lambda(e^{iu}-1)).
    \end{equation*}
    Thus the result follows.
\end{proof}


\end{document}
